\section{Rules}

\subsection{\textsf{map}}
As it turns out we need two \textsf{map} rules.

\begin{definition}[\textsf{map$_\textsf{a}$}]
\begin{eqnarray*}[x]
  \begin{eqnalign}[lcl]
    \mathcal{C}[\ol{x}\ \ttt{::}\ \ttt{xs}] &=>& \mathbb{D}(\mathcal{C}[\ol{x}])\
    \ttt{::}\ \ttt{self}(\mathcal{C}[\ttt{xs}]) \\
    \mathcal{D} &=>& \ttt{nil} \\
  \end{eqnalign}\\
  \textsf{where}\ \textsf{samedom} (\mathcal{C}, \mathcal{D}) \\
%
  \Downarrow \\
%
  \begin{eqnalign}[lcl]
    \mathcal{C}[\ttt{xs}] &=>& \ttt{map (fn x => $\mathbb{D}(
    \mathcal{C}[$x$])$)} \ \ttt{xs} \\
  \end{eqnalign}
 \end{eqnarray*}
\end{definition}

\begin{definition}[\textsf{map$_\textsf{b}$}]
\begin{eqnarray*}[x]
  \begin{eqnalign}[lcl]
    \mathcal{C}[\ol{x}\ \ttt{::}\ \ttt{xs}] &=>& \mathbb{D}(\mathcal{C}[\ol{x}])\
    \ttt{::}\ \ttt{self}(\mathcal{C}[\ttt{xs}]) \\
    \mathcal{C}[\ttt{x}] &=>& \ttt{x} \\
  \end{eqnalign}\\
%
  \Downarrow \\
%
  \begin{eqnalign}[lcl]
    \mathcal{C}[\ttt{xs}] &=>& \ttt{map (fn x => $\mathbb{D}(
    \mathcal{C}[$x$])$)} \ \ttt{xs} \\
  \end{eqnalign}
 \end{eqnarray*}
\end{definition}
To see the need for two rules consider the two functions
\begin{multicols}{2}
\begin{sml}
fun f (x :: xs) = x + 42 :: f xs
  | f nil       = nil
\end{sml}
\begin{sml}
fun g (x :: xs) = x + 42 :: g xs
  | g _         = nil
\end{sml}
\end{multicols}
Their normal forms are
\begin{multicols}{2}
\begin{sml}
fun f (x :: xs) = x + 42 :: f xs
  | f x         = x
\end{sml}
\begin{sml}
fun g (x :: xs) = x + 42 :: g xs
  | g x         = nil
\end{sml}
\end{multicols}
Which is essentially why we need two rules.

\subsection{\textsf{foldr}}

\begin{definition}[\textsf{foldr}]
\begin{eqnarray*}[x]
  \begin{eqnalign}[lcl]
    \mathcal{C}[\ol{x}\ \ttt{::}\ \ttt{xs}] &=>& \mathbb{D}(\mathcal{C}[\ol{x}],\
    \ttt{self}(\mathcal{C}[\ttt{xs}]))\\
    \mathcal{D} &=>& \mathbb{E}(\mathcal{D})
  \end{eqnalign}\\
  \textsf{where}\ \textsf{samedom}(\mathcal{C}, \mathcal{D}) \\
%
  \Downarrow \\
%
  \begin{eqnalign}[lcl]
    \mathcal{C}[\ttt{xs}] &=>& \ttt{foldr (fn (x, a) =>
      $\mathbb{D}(\mathcal{C}[$x$],\ $a$)$) ($\mathbb{E}(\mathcal{C}[$xs$])$) \ttt{xs}}
  \end{eqnalign}
 \end{eqnarray*}
\end{definition}

\subsection{\textsf{foldl}}

\begin{definition}[\textsf{foldl}]
\begin{eqnarray*}[x]
  \begin{eqnalign}[lcl]
    \mathcal{C}[\ol{x}\ \ttt{::}\ \ttt{xs}][\ol{a}] &=>&
    \ttt{self}(\mathcal{C}[\ol{x}][\mathbb{D}(\mathcal{C}[\ol{x}][\ol{a}])])\\
    \mathcal{C}[\ol{x}][\ol{a}] &=>& \ol{a}
  \end{eqnalign}\\
%
  \Downarrow \\
%
  \begin{eqnalign}[lcl]
    \mathcal{C}[\ttt{xs}][\ttt{a}] &=>& \ttt{foldl (fn (x, a) =>
      $\mathbb{D}(\mathcal{C}[$x$][$a$])$) \ttt{a} \ttt{xs}}
  \end{eqnalign}
 \end{eqnarray*}
\end{definition}

%%% Local Variables: 
%%% mode: latex
%%% TeX-master: "../report"
%%% End: 
